thesis/fault-modelling-theory/BoolOperand.thy
@@ -1,0 +1,30 @@
+theory BoolOperand
+
+imports Main FaultModellingTypes
+
+begin
+
+primrec "BoolOperand_eval" :: "'vb BoolOperand \<Rightarrow> ('vb \<Rightarrow> bool) \<Rightarrow> bool" where
+  "BoolOperand_eval (VBBConstOp b) vb = b" |
+  "BoolOperand_eval (VBBVarOp a) vb = vb a" |
+  "BoolOperand_eval (VBBExpUnOp exp_op op1) vb = exp_op (BoolOperand_eval op1 vb)" |
+  "BoolOperand_eval (VBBExpBinOp exp_op op1 op2) vb = 
+    exp_op (BoolOperand_eval op1 vb) (BoolOperand_eval op2 vb)"
+
+primrec 
+  expand_BoolOperand_ValuesOperand :: "'vb BoolOperand \<Rightarrow> ('vb, 'vv) ValuesOperand \<Rightarrow> ('vb, 'vv) ValuedBool list" and
+  expand_BoolOperand_ValuesOperand_list :: "'vb BoolOperand \<Rightarrow> ('vb, 'vv) ValuedBool list \<Rightarrow> ('vb, 'vv) ValuedBool list" and
+  expand_BoolOperand_ValuesOperand_VB :: "'vb BoolOperand \<Rightarrow> ('vb, 'vv) ValuedBool \<Rightarrow> ('vb, 'vv) ValuedBool"
+where
+  "expand_BoolOperand_ValuesOperand e (VBVConstOp c) = (VB e (VBVConstOp c)) # []" |
+  "expand_BoolOperand_ValuesOperand e (VBVVarOp v) = (VB e (VBVVarOp v)) # []" |
+  expand_BoolOperand_ValuesOperand_VBExpOp:
+  "expand_BoolOperand_ValuesOperand e (VBVExpOp Es) = expand_BoolOperand_ValuesOperand_list e Es" |
+  "expand_BoolOperand_ValuesOperand_list e [] = []" |
+  "expand_BoolOperand_ValuesOperand_list e (E # Es) = 
+    (expand_BoolOperand_ValuesOperand_VB e E) # (expand_BoolOperand_ValuesOperand_list e Es)" |
+  "expand_BoolOperand_ValuesOperand_VB e1 (VB e2 v2) = VB (VBBExpBinOp (op \<and>) e1 e2) v2"
+
+(* FAZER O NORMALISE DE BOOLEANO PARA SUPORTAR A EQUIVALENCIA DE ÁRVORE COM BOOLEANO *)
+
+end
